examples/proofs/paper_example_2_1/generated_spec.v
@@ -92,6 +92,11 @@ Section spec.
     fn(∀ (a, n, p) : nat * nat * loc; (p @ (&own (a @ (mem_t)))), (n @ (int (size_t))); True)
       → ∃ () : (), ((n ≤ a) @ (optional (&own (uninit (n))) (null))); (p ◁ₗ ((n ≤ a ? a - n : a) @ (mem_t))).
 
+  (* Specifications for function [alloc_from_start]. *)
+  Definition type_of_alloc_from_start :=
+    fn(∀ (a, n, p) : nat * nat * loc; (p @ (&own (a @ (mem_t)))), (n @ (int (size_t))); True)
+      → ∃ () : (), ((n ≤ a) @ (optional (&own (uninit (n))) (null))); (p ◁ₗ ((n ≤ a ? a - n : a) @ (mem_t))).
+
   (* Specifications for function [thread_safe_alloc]. *)
   Definition type_of_thread_safe_alloc :=
     fn(∀ (lid, n) : lock_id * nat; (n @ (int (size_t))); (initialized "lock" lid) ∗ (initialized "data" lid))
