examples/proofs/paper_example_2_1/generated_proof_alloc_from_start.v
@@ -5,24 +5,24 @@ From refinedc.examples.spinlock Require Import spinlock_def.
 Set Default Proof Using "Type".
 
 (* Generated from [examples/paper_example_2_1.c]. *)
-Section proof_alloc.
+Section proof_alloc_from_start.
   Context `{!typeG Σ} `{!globalG Σ}.
   Context `{!lockG Σ}.
 
-  (* Typing proof for [alloc]. *)
-  Lemma type_alloc :
-    ⊢ typed_function impl_alloc type_of_alloc.
+  (* Typing proof for [alloc_from_start]. *)
+  Lemma type_alloc_from_start :
+    ⊢ typed_function impl_alloc_from_start type_of_alloc_from_start.
   Proof.
     Open Scope printing_sugar.
-    start_function "alloc" ([[a n] p]) => arg_d arg_sz.
+    start_function "alloc_from_start" ([[a n] p]) => arg_d arg_sz local_res.
     split_blocks ((
       ∅
     )%I : gmap label (iProp Σ)) ((
       ∅
     )%I : gmap label (iProp Σ)).
     - repeat liRStep; liShow.
-      all: print_typesystem_goal "alloc" "#0".
+      all: print_typesystem_goal "alloc_from_start" "#0".
     Unshelve. all: sidecond_hook; prepare_sideconditions; normalize_and_simpl_goal; try solve_goal; unsolved_sidecond_hook.
-    all: print_sidecondition_goal "alloc".
+    all: print_sidecondition_goal "alloc_from_start".
   Qed.
-End proof_alloc.
+End proof_alloc_from_start.
